[Dafny] Reorganize files

compiler/dafny/semantics/dafny_eval_relScript.sml
@@ -14,13 +14,29 @@ val _ = new_theory "dafny_eval_rel";
 Overload True = “Lit (BoolL T)”;
 Overload False = “Lit (BoolL F)”;
 
-Overload "imp" = “BinOp Imp”
+Overload "not" = “UnOp Not”;
+Overload "imp" = “BinOp Imp”;
+Overload "dfy_eq" = “BinOp Eq”;
 
 Definition eval_exp_def:
   eval_exp st env e v ⇔
     ∃ck1 ck2.
       evaluate_exp (st with clock := ck1) env e =
         (st with clock := ck2, Rval v)
+End
+
+Definition eval_rhs_exp_def:
+  eval_rhs_exp st env e st' v ⇔
+    ∃ck1 ck2.
+      evaluate_rhs_exp (st with clock := ck1) env e =
+        (st' with clock := ck2, Rval v)
+End
+
+Definition eval_rhs_exps_def:
+  eval_rhs_exps st env es st' vs ⇔
+    ∃ck1 ck2.
+      evaluate_rhs_exps (st with clock := ck1) env es =
+        (st' with clock := ck2, Rval vs)
 End
 
 Definition eval_stmt_def:
@@ -37,8 +53,15 @@ End
 Definition valid_def:
   valid e = ∀st env. eval_true st env e
 End
-
 Overload "⊢" = “valid”;
+
+Definition CanEval_def: (* beautiful or not.. *)
+  CanEval e = dfy_eq e e
+End
+
+Definition IsBool_def:
+  IsBool e = CanEval $ dfy_eq e True
+End
 
 Definition conj_def:
   conj [] = Lit (BoolL T) ∧
@@ -59,6 +82,12 @@ Theorem conj_empty[simp]:
   conj [] = True
 Proof
   rewrite_tac [conj_def]
+QED
+
+Triviality value_same_type_same_value[simp]:
+  value_same_type v v
+Proof
+  Cases_on ‘v’ \\ gvs [value_same_type_def]
 QED
 
 (* *** *)
@@ -133,6 +162,289 @@ Proof
   \\ dxrule (cj 2 evaluate_exp_add_to_clock) \\ simp []
   \\ disch_then $ qspec_then ‘ck₂’ assume_tac
   \\ qexistsl [‘ck₁ + ck₃’, ‘ck₂ + ck₄’] \\ gvs []
+QED
+
+Theorem eval_true_CanEval:
+  eval_true st env (CanEval e) ⇒ ∃v. eval_exp st env e v
+Proof
+  gvs [eval_true_def,CanEval_def,evaluate_exp_def,eval_exp_def]
+  \\ gvs [AllCaseEqs(),PULL_EXISTS,do_sc_def,do_bop_def]
+  \\ gvs []
+  \\ rpt strip_tac
+  \\ rev_drule (cj 1 evaluate_exp_with_clock)
+  \\ disch_then $ qx_choose_then ‘ck’ assume_tac \\ gvs []
+  \\ last_assum $ irule_at Any
+QED
+
+Theorem EVERY_eval_true_CanEval:
+  EVERY (eval_true st env) (MAP CanEval args) ⇒
+  ∃in_vs. LIST_REL (eval_exp st env) args in_vs
+Proof
+  Induct_on ‘args’ \\ gvs [] \\ rw []
+  \\ res_tac \\ drule eval_true_CanEval \\ strip_tac
+  \\ rpt $ pop_assum $ irule_at Any
+QED
+
+Theorem eval_exp_not_not:
+  eval_exp st env (not (not x)) (BoolV b) ⇒ eval_exp st env x (BoolV b)
+Proof
+  strip_tac
+  \\ gvs [eval_exp_def, evaluate_exp_def, do_uop_def, AllCaseEqs()]
+  \\ last_x_assum $ irule_at (Pos hd)
+QED
+
+Theorem eval_exp_bool_not:
+  eval_exp st env a (BoolV b) ⇒ eval_exp st env (not a) (BoolV ¬b)
+Proof
+  strip_tac
+  \\ gvs [eval_exp_def, evaluate_exp_def, do_uop_def, PULL_EXISTS, AllCaseEqs()]
+  \\ last_x_assum $ irule_at (Pos hd)
+QED
+
+Theorem eval_true_isbool:
+  eval_true st env (IsBool a) ⇒ ∃b. eval_exp st env a (BoolV b)
+Proof
+  strip_tac
+  \\ gvs [eval_true_def, eval_exp_def, IsBool_def, CanEval_def,
+          evaluate_exp_def, do_sc_def, do_bop_def, value_same_type_def,
+          AllCaseEqs()]
+  \\ imp_res_tac evaluate_exp_with_clock \\ gvs []
+  \\ rename [‘_ ⇔ v₀ = _’]
+  \\ Cases_on ‘v₀’ \\ gvs []
+  \\ last_x_assum $ irule_at (Pos hd)
+QED
+
+Theorem eval_true_isbool_cases:
+  eval_true st env (IsBool a) ⇒
+  eval_true st env a ∨ eval_true st env (not a)
+Proof
+  strip_tac
+  \\ drule eval_true_isbool
+  \\ disch_then $ qx_choose_then ‘b’ assume_tac
+  \\ Cases_on ‘b’
+  \\ gvs [eval_true_def]
+  \\ drule eval_exp_bool_not \\ simp []
+QED
+
+Theorem eval_true_imp:
+  eval_true st env (imp a b) ⇒
+  (eval_true st env a ⇒ eval_true st env b)
+Proof
+  simp [eval_true_def, eval_exp_def, PULL_EXISTS, PULL_FORALL]
+  \\ qx_genl_tac [‘ck₁’, ‘ck₂’, ‘ck₃’, ‘ck₄’]
+  \\ rpt strip_tac
+  \\ rev_dxrule (cj 1 evaluate_exp_add_to_clock) \\ simp []
+  \\ disch_then $ qspec_then ‘ck₃’ assume_tac
+  \\ rev_dxrule (cj 1 evaluate_exp_add_to_clock) \\ simp []
+  \\ disch_then $ qspec_then ‘ck₁’ assume_tac
+  \\ gvs [evaluate_exp_def]
+  \\ gvs [do_sc_def, do_bop_def, AllCaseEqs()]
+  \\ last_x_assum $ irule_at (Pos hd)
+QED
+
+Theorem eval_stmt_Skip:
+  eval_stmt st env Skip st Rcont
+Proof
+  gvs [eval_stmt_def, evaluate_stmt_def, state_component_equality]
+QED
+
+Theorem eval_stmt_Assert:
+  eval_true st env e
+  ⇒
+  eval_stmt st env (Assert e) st Rcont
+Proof
+  strip_tac
+  \\ gvs [eval_stmt_def, evaluate_stmt_def]
+  \\ Cases_on ‘env.is_running’ \\ simp []
+  >- (gvs [state_component_equality])
+  \\ gvs [eval_true_def, eval_exp_def, AllCaseEqs()]
+  \\ last_assum $ irule_at (Pos hd)
+QED
+
+Theorem eval_stmt_Return:
+  eval_stmt st env Return st (Rstop Sret)
+Proof
+  gvs [eval_stmt_def, evaluate_stmt_def, state_component_equality]
+QED
+
+Theorem eval_stmt_Then_cont:
+  eval_stmt st env stmt₁ st₁ Rcont ∧
+  eval_stmt st₁ env stmt₂ st₂ Rcont
+  ⇒
+  eval_stmt st env (Then stmt₁ stmt₂) st₂ Rcont
+Proof
+  strip_tac
+  \\ gvs [eval_stmt_def]
+  \\ rename
+       [‘evaluate_stmt (_ with clock := ck₃) _ _ = (_ with clock := ck₄, _)’]
+  \\ pop_assum mp_tac
+  \\ rename
+       [‘evaluate_stmt (_ with clock := ck₁) _ _ = (_ with clock := ck₂, _)’]
+  \\ disch_tac
+  \\ rev_dxrule evaluate_stmt_add_to_clock \\ simp []
+  \\ disch_then $ qspec_then ‘ck₃’ assume_tac
+  \\ rev_dxrule evaluate_stmt_add_to_clock \\ simp []
+  \\ disch_then $ qspec_then ‘ck₂’ assume_tac
+  \\ simp [evaluate_stmt_def, AllCaseEqs()]
+  \\ last_x_assum $ irule_at (Pos hd)
+  \\ gvs [state_component_equality]
+QED
+
+Theorem eval_stmt_Then_ret:
+  eval_stmt st env stmt₁ st₁ (Rstop Sret)
+  ⇒
+  eval_stmt st env (Then stmt₁ stmt₂) st₁ (Rstop Sret)
+Proof
+  strip_tac
+  \\ gvs [eval_stmt_def, evaluate_stmt_def, AllCaseEqs()]
+  \\ last_assum $ irule_at (Pos hd) \\ simp [state_component_equality]
+QED
+
+Theorem eval_stmt_Then_cont_ret:
+  eval_stmt st env stmt₁ st₁ Rcont ∧
+  eval_stmt st₁ env stmt₂ st₂ (Rstop Sret)
+  ⇒
+  eval_stmt st env (Then stmt₁ stmt₂) st₂ (Rstop Sret)
+Proof
+  strip_tac
+  \\ gvs [eval_stmt_def]
+  \\ rename
+       [‘evaluate_stmt (_ with clock := ck₃) _ _ = (_ with clock := ck₄, _)’]
+  \\ pop_assum mp_tac
+  \\ rename
+       [‘evaluate_stmt (_ with clock := ck₁) _ _ = (_ with clock := ck₂, _)’]
+  \\ disch_tac
+  \\ rev_dxrule evaluate_stmt_add_to_clock \\ simp []
+  \\ disch_then $ qspec_then ‘ck₃’ assume_tac
+  \\ rev_dxrule evaluate_stmt_add_to_clock \\ simp []
+  \\ disch_then $ qspec_then ‘ck₂’ assume_tac
+  \\ simp [evaluate_stmt_def, AllCaseEqs()]
+  \\ last_x_assum $ irule_at (Pos hd)
+  \\ gvs [state_component_equality]
+QED
+
+Theorem eval_stmt_If_thn:
+  eval_true st env grd ∧
+  eval_stmt st env thn st₁ ret ∧
+  ret ≠ Rstop (Serr Rtimeout_error)
+  ⇒
+  eval_stmt st env (If grd thn els) st₁ ret
+Proof
+  gvs [eval_stmt_def, eval_true_def, eval_exp_def, PULL_EXISTS]
+  \\ qx_genl_tac [‘ck₁’, ‘ck₂’, ‘ck₃’, ‘ck₄’]
+  \\ strip_tac
+  \\ simp [evaluate_stmt_def]
+  \\ dxrule (cj 1 evaluate_exp_add_to_clock) \\ gvs []
+  \\ disch_then $ qspec_then ‘ck₃’ assume_tac
+  \\ dxrule evaluate_stmt_add_to_clock \\ gvs []
+  \\ disch_then $ qspec_then ‘ck₂’ assume_tac
+  \\ qexists ‘ck₁ + ck₃’ \\ gvs []
+  \\ simp [do_cond_def, state_component_equality]
+QED
+
+Theorem eval_stmt_If_els:
+  eval_true st env (not grd) ∧
+  eval_stmt st env els st₁ ret ∧
+  ret ≠ Rstop (Serr Rtimeout_error)
+  ⇒
+  eval_stmt st env (If grd thn els) st₁ ret
+Proof
+  gvs [eval_stmt_def, eval_true_def]
+  \\ strip_tac
+  \\ dxrule_then assume_tac eval_exp_bool_not
+  \\ dxrule_then assume_tac eval_exp_not_not \\ gvs []
+  \\ gvs [eval_exp_def]
+  \\ rename
+       [‘evaluate_exp (_ with clock := ck₁) _ _ = (_ with clock := ck₂, _)’,
+        ‘evaluate_stmt (_ with clock := ck₃) _ _ = (_ with clock := ck₄, _)’]
+  \\ simp [evaluate_stmt_def]
+  \\ dxrule (cj 1 evaluate_exp_add_to_clock) \\ gvs []
+  \\ disch_then $ qspec_then ‘ck₃’ assume_tac
+  \\ dxrule evaluate_stmt_add_to_clock \\ gvs []
+  \\ disch_then $ qspec_then ‘ck₂’ assume_tac
+  \\ qexists ‘ck₁ + ck₃’ \\ gvs []
+  \\ simp [do_cond_def, state_component_equality]
+QED
+
+Theorem eval_stmt_Assign:
+  eval_rhs_exps st env (MAP SND ass) st₁ vs ∧
+  assign_values st₁ env (MAP FST ass) vs = (st', Rcont)
+  ⇒
+  eval_stmt st env (Assign ass) st' Rcont
+Proof
+  strip_tac
+  \\ simp [eval_stmt_def, evaluate_stmt_def]
+  \\ fs [eval_rhs_exps_def, PULL_EXISTS, AllCaseEqs()]
+  \\ dxrule evaluate_rhs_exps_add_to_clock \\ simp []
+  \\ disch_then $ qspec_then ‘st₁.clock’ assume_tac
+  \\ last_x_assum $ irule_at (Pos hd)
+  \\ dxrule assign_values_add_to_clock \\ simp []
+  \\ simp [state_component_equality]
+QED
+
+Theorem eval_stmt_MetCall:
+  get_member mname env.prog =
+    SOME (Method name ins reqs ens rds decrs outs mods body) ∧
+  LIST_REL (eval_exp st env) args in_vs ∧
+  set_up_call st (MAP FST ins) in_vs (MAP FST outs) = SOME st₁ ∧
+  eval_stmt st₁ env body st₂ (Rstop Sret) ∧
+  OPT_MMAP (read_local st₂.locals) (MAP FST outs) = SOME out_vs ∧
+  LENGTH rets = LENGTH out_vs ∧
+  assign_values (restore_caller st₂ st) env rets out_vs = (st',Rcont)
+  ⇒
+  eval_stmt st env (MetCall rets mname args) st' Rcont
+Proof
+  rpt strip_tac
+  \\ simp [eval_stmt_def, evaluate_stmt_def]
+  \\ dxrule_then mp_tac eval_exp_evaluate_exps
+  \\ disch_then $ qx_choosel_then [‘ck’, ‘ck₁’] assume_tac \\ simp []
+  \\ fs [eval_stmt_def]
+  \\ rename
+       [‘evaluate_stmt (_ with clock := ck₂) _ _ = (_ with clock := ck₃, _)’]
+  \\ qexists ‘st₂.clock + ck + ck₂ + 1’
+  \\ dxrule (cj 2 evaluate_exp_add_to_clock) \\ simp []
+  \\ disch_then assume_tac
+  \\ qmatch_goalsub_abbrev_tac ‘set_up_call (_ with clock := ck₄)’
+  \\ dxrule set_up_call_some_with_clock
+  \\ disch_then assume_tac
+  \\ simp [Abbr ‘ck₄’, dec_clock_def]
+  \\ dxrule evaluate_stmt_add_to_clock \\ simp []
+  \\ disch_then $ qspec_then ‘ck₁ + st₂.clock’ assume_tac \\ gvs []
+  \\ rewrite_tac [restore_caller_cur_with_clock, restore_caller_prev_with_clock]
+  \\ dxrule assign_values_add_to_clock \\ simp []
+  \\ disch_then $ qspec_then ‘ck₁ + ck₃’ assume_tac \\ gvs []
+  \\ simp [state_component_equality]
+QED
+
+Theorem eval_stmt_Rcont_old:
+  eval_stmt st env stmt st' Rcont ⇒
+  st'.locals_old = st.locals_old ∧ st'.heap_old = st.heap_old
+Proof
+  simp [eval_stmt_def] \\ strip_tac
+  \\ imp_res_tac evaluate_stmt_Rcont_old \\ gvs []
+QED
+
+Triviality eval_exp_old_eq:
+  st₁.locals_old = st.locals_old ∧ st₁.heap_old = st.heap_old ∧
+  eval_exp st₁ env (Old e) v ⇒
+  eval_exp st env (Old e) v
+Proof
+  strip_tac
+  \\ gvs [eval_exp_def]
+  \\ drule evaluate_exp_old_Rval_eq \\ gvs []
+  \\ disch_then $ qspec_then ‘st’ mp_tac \\ simp []
+  \\ disch_then $ qx_choosel_then [‘ck’, ‘st'’] assume_tac
+  \\ qexists ‘ck’ \\ gvs []
+  \\ imp_res_tac evaluate_exp_with_clock
+  \\ gvs [state_component_equality]
+QED
+
+Theorem eval_exp_old_eq:
+  st₁.locals_old = st.locals_old ∧ st₁.heap_old = st.heap_old ⇒
+  eval_exp st₁ env (Old e) v =
+  eval_exp st env (Old e) v
+Proof
+  metis_tac [eval_exp_old_eq]
 QED
 
 val _ = export_theory ();
